Fomega/Basic/Inversion.lean
@@ -47,11 +47,41 @@ namespace Fomega.Proof
         subst e1; subst e2; subst e3
         apply @ih1 A B K (Term.RedConv.trans h3 hc) rfl
 
-  theorem lam_destruct :
+  theorem lam_destruct_conv :
     Γ ⊢ .lam mf A t : T ->
-    Γ ⊢ .all mf C B : .const K ->
-    T =β= .all mf C B ->
-    A =β= C ∧ (A::Γ) ⊢ t : B
+    T =β= .all mf C D ->
+    ∃ B, A =β= C ∧ B =β= D ∧ Γ ⊢ .lam mf A t : .all mf A B
+  := by
+  intro j hc
+  generalize sdef : Term.lam mf A t = s at *
+  induction j generalizing A C D t
+  case ax => simp at sdef
+  case var => simp at sdef
+  case pi => simp at sdef
+  case tpi => simp at sdef
+  case lam A' B' K' t' j3 j4 ih1 ih2 =>
+    replace hc := Term.RedConv.all_congr hc
+    injection sdef with e1 e2 e3
+    subst e2; subst e3; exists B'
+    apply And.intro hc.2.1
+    apply And.intro hc.2.2
+    constructor; apply j3; apply j4
+  case app => simp at sdef
+  case conv Γ t' A' B' _K' h1 _h2 h3 ih1 _ih2 =>
+    cases t' <;> simp at sdef
+    case _ m r1 r2 =>
+      cases sdef
+      case _ e1 sdef =>
+      cases sdef
+      case _ e2 e3 =>
+        subst e1; subst e2; subst e3
+        apply @ih1 A t C D (Term.RedConv.trans h3 hc) rfl
+
+  theorem lam_destruct_body :
+    Γ ⊢ .lam mf A t : T ->
+    Γ ⊢ .all mf A B : .const K ->
+    T =β= .all mf A B ->
+    (A::Γ) ⊢ t : B
   := by
   intro j1 j2 hc
   generalize sdef : Term.lam mf A t = s at *
@@ -65,8 +95,8 @@ namespace Fomega.Proof
     subst e2; subst e3
     replace j3 := all_destruct j2 Term.RedConv.refl
     have lem := Term.RedConv.all_congr hc
-    apply And.intro; apply lem.2.1
-    apply Proof.conv; apply j4; repeat sorry
+    apply Proof.conv; apply j4
+    apply j3.2.2; apply lem.2.2
   case app => simp at sdef
   case conv Γ t' A' B' _K' h1 _h2 h3 ih1 _ih2 =>
     cases t' <;> simp at sdef
@@ -77,6 +107,5 @@ namespace Fomega.Proof
       case _ e2 e3 =>
         subst e1; subst e2; subst e3
         apply @ih1 A t B K j2 (Term.RedConv.trans h3 hc) rfl
-
 
 end Fomega.Proof
