Fomega/Basic/Preservation.lean
@@ -9,35 +9,113 @@ import Fomega.Basic.Classification
 
 namespace Fomega.Proof
 
-  theorem conv_ctx : t ⊢ Γ -> Γ ⊢ t : A ->
-    (∀ n, Γ d@ n =β= Δ d@ n) ->
-    t ⊢ Δ ∧ Δ ⊢ t : A
-  := by
-  intro cj j h
-  sorry
+  -- theorem wf_type_conv : A ⊢ Γ -> A =β= B -> Γ ⊢ B : .const K -> B ⊢ Γ := by
+  -- intro wf cv j
+  -- induction wf generalizing B K
 
-  theorem preservation1 : Γ ⊢ t : A -> t -β> t' -> Γ ⊢ t' : A := by
-  intro j r
+  -- theorem wf_type2 : t ⊢ Γ -> Γ ⊢ t : A -> A ⊢ Γ := by
+  -- intro j1 j2
+  -- induction j1 generalizing A
+  -- case ax => sorry
+  -- case var Γ x K j3 j4 ih =>
+  --   generalize sdef : Term.bound K x = s at *
+  --   induction s generalizing K x
+  --   all_goals try cases sdef
+  --   case _ K i =>
+  -- case pi => sorry
+  -- case lam => sorry
+  -- case app => sorry
+
+  theorem wf_type : t ⊢ Γ -> Γ ⊢ t : A -> A ⊢ Γ := by
+  intro j1 j2
+  induction j2
+  case ax => constructor
+  case var => cases j1; simp [*]
+  case pi => constructor
+  case tpi => constructor
+  case lam => sorry
+  case app => sorry
+  case conv j2 cv ih _ => sorry
+
+  theorem preservation1 : t ⊢ Γ -> Γ ⊢ t : A -> t -β> t' -> Γ ⊢ t' : A := by
+  intro cj j r
   induction j generalizing t'
   case ax => cases r
   case var => cases r
   case pi => sorry
   case tpi => sorry
-  case lam => sorry
+  case lam Γ A K t B j1 j2 ih1 ih2 =>
+    cases r
+    case lam_congr1 A' r => sorry
+    case lam_congr2 => sorry
   case app Γ f A' B a B' j1 j2 j3 ih1 ih2 =>
     cases r
-    case beta C d => sorry
+    case beta C d =>
+      have j4 := lam_destruct_conv j1 Term.RedConv.refl
+      cases j4
+      case _ B2 j4 =>
+      cases cj
+      case _ cj1 cj2 =>
+        have cl := proof_classification cj1 j4.2.2
+        cases cl
+        case _ h => cases h
+        case _ h =>
+        cases h
+        case _ K j5 =>
+          have j6 := lam_destruct_body j4.2.2 j5 Term.RedConv.refl
+          have cl2 := proof_classification cj1 j1
+          cases cl2
+          case _ h => cases h
+          case _ h =>
+          cases h
+          case _ K2 j7 =>
+            have lem1 : Γ ⊢ a : C := by
+              replace j5 := all_destruct j5 Term.RedConv.refl
+              cases j5.2.1
+              case _ K3 j8 =>
+                apply Proof.conv; apply j2; apply j8
+                apply Term.RedConv.sym j4.1
+            have lem2 : B2 β[a] =β= B β[a] := by
+              apply Term.RedConv.subst; apply j4.2.1
+            have lem3 : Γ ⊢ (B β[a]) : Term.const K2 := by
+              replace j7 := all_destruct j7 Term.RedConv.refl
+              have j8 := beta j7.2.2 j2
+              apply j8
+            replace j6 := beta j6 lem1
+            apply Proof.conv; apply j6; rw [j3]; apply lem3
+            rw [j3]; apply lem2
     case app_congr1 => sorry
     case app_congr2 => sorry
   case conv j1 j2 j3 ih1 ih2 =>
-    apply Proof.conv; apply ih1 r
+    apply Proof.conv; apply ih1 cj r
     apply j2; apply j3
 
-  theorem preservation : Γ ⊢ t : A -> t -β>* t' -> Γ ⊢ t' : A := by
-  intro j r
-  induction r generalizing Γ A
-  case _ => exact j
-  case _ r1 _r2 ih => apply ih (preservation1 j r1)
+  theorem preservation_wf1 : t ⊢ Γ -> Γ ⊢ t : A -> t -β> t' -> t' ⊢ Γ := by
+  intro j1 j2 r
+  induction j2 generalizing t'
+  case ax => cases r
+  case var => cases r
+  case pi => sorry
+  case tpi => sorry
+  case lam => sorry
+  case app j2 j3 j4 ih1 ih2 =>
+    cases j1
+    case _ cj1 cj2 =>
+    cases r
+    case beta =>
+      cases cj1
+      case _ cj1 cj3 =>
+        sorry
+    case app_congr1 => sorry
+    case app_congr2 => sorry
+  case conv ih1 ih2 => apply ih1 j1 r
+
+
+  -- theorem preservation : Γ ⊢ t : A -> t -β>* t' -> Γ ⊢ t' : A := by
+  -- intro j r
+  -- induction r generalizing Γ A
+  -- case _ => exact j
+  -- case _ r1 _r2 ih => apply ih (preservation1 j r1)
 
   theorem preservation_type : Γ ⊢ t : A -> A -β>* A' -> Γ ⊢ t : A' := by sorry
 
