Fomega/Basic/Substitution.lean
@@ -39,6 +39,19 @@ namespace Fomega.Proof
       rw [<-Term.subst_apply_compose_commute]
       apply weaken; exact h1
 
+  theorem lift_subst_replace_wf :
+    (∀ n t, σ n = .replace t -> t ⊢ Δ) ->
+    (∀ n t, ^σ n = .replace t -> t ⊢ ([σ]A :: Δ))
+  := by
+  intro h1 n t h2
+  cases n <;> simp at *
+  case _ n =>
+    unfold Term.Subst.compose at h2; simp at h2
+    generalize ydef : σ n = y at *
+    cases y <;> simp at h2
+    case _ t' =>
+      rw [<-h2]; apply weaken_wf; apply h1 n t' ydef
+
   theorem subst :
     (∀ n t, σ n = .replace t -> IsPreProof t) ->
     (∀ n y, σ n = .rename y -> [σ](Γ d@ n) = Δ d@ y) ->
@@ -72,6 +85,38 @@ namespace Fomega.Proof
     constructor; apply ih1 h1 h2 h3; apply ih2 h1 h2 h3
     apply Term.RedConv.subst _ j3
 
+  theorem subst_wf :
+    (∀ n t, σ n = .replace t -> IsPreProof t) ->
+    (∀ n y, σ n = .rename y -> [σ](Γ d@ n) = Δ d@ y) ->
+    (∀ n t, σ n = .replace t -> Δ ⊢ t : ([σ]Γ d@ n)) ->
+    (∀ n t, σ n = .replace t -> t ⊢ Δ) ->
+    t ⊢ Γ -> ([σ]t) ⊢ Δ
+  := by
+  intro h1 h2 h3 h4 j
+  induction j generalizing Δ σ
+  case _ => constructor
+  case var Γ x K j1 _j2 ih =>
+    simp; generalize ydef : σ x = y at *
+    cases y <;> simp
+    case _ y =>
+      constructor
+      replace j := subst h1 h2 h3 j1
+      rw [h2 _ _ ydef] at j; simp at j; exact j
+      replace ih := ih h1 h2 h3 h4; rw [h2 _ _ ydef] at ih; exact ih
+    case _ t' => apply h4 _ _ ydef
+  case pi A Γ B _ _ ih1 ih2 =>
+    simp; constructor; apply ih1 h1 h2 h3 h4
+    replace ih2 := @ih2 (^σ) ([σ]A::Δ) (IsPreProof.lift h1) (lift_subst_rename h2)
+      (lift_subst_replace h3) (lift_subst_replace_wf h4)
+    simp at ih2; exact ih2
+  case lam A Γ B _ _ ih1 ih2 =>
+    simp; constructor; apply ih1 h1 h2 h3 h4
+    replace ih2 := @ih2 (^σ) ([σ]A::Δ) (IsPreProof.lift h1) (lift_subst_rename h2)
+      (lift_subst_replace h3) (lift_subst_replace_wf h4)
+    simp at ih2; exact ih2
+  case app ih1 ih2 =>
+    simp; constructor; apply ih1 h1 h2 h3 h4; apply ih2 h1 h2 h3 h4
+
   theorem beta : (A::Γ) ⊢ b : B -> Γ ⊢ t : A -> Γ ⊢ (b β[t]) : (B β[t]) := by
   simp; intro j1 j2
   apply @subst _ (A::Γ)
@@ -82,12 +127,32 @@ namespace Fomega.Proof
   case _ =>
     intro n y h
     cases n <;> simp at h
-    case _ n =>
-      subst h; simp
+    case _ n => subst h; simp
   case _ =>
     intro n t' h
     cases n <;> simp at h
     case _ => subst h; simp; exact j2
+  case _ => exact j1
+
+  theorem beta_wf : b ⊢ (A::Γ) -> Γ ⊢ t : A -> t ⊢ Γ -> (b β[t]) ⊢ Γ := by
+  simp; intro j1 j2 j3
+  apply @subst_wf _ (A::Γ)
+  case _ =>
+    intro n s eq
+    cases n <;> simp at *
+    subst eq; apply IsPreProof.from_proof j2
+  case _ =>
+    intro n y h
+    cases n <;> simp at h
+    case _ n => subst h; simp
+  case _ =>
+    intro n t' h
+    cases n <;> simp at h
+    case _ => subst h; simp; exact j2
+  case _ =>
+    intro n t' h
+    cases n <;> simp at h
+    case _ => subst h; exact j3
   case _ => exact j1
 
 end Fomega.Proof
